PropositionalLogic/Sound_Classical_Trivial.v
@@ -1,0 +1,155 @@
+Require Import Logic.LogicBase.
+Require Import Logic.PropositionalLogic.Syntax.
+Require Import Logic.PropositionalLogic.ClassicalPropositionalLogic.
+Require Import Logic.PropositionalLogic.TrivialSemantics.
+
+Local Open Scope logic_base.
+Local Open Scope PropositionalLogic.
+
+Lemma sound_ImpNegAsPrime {Var: Type}:
+  forall x y: @expr (PropositionalLanguage.L Var),
+    ImpNegAsPrime.atomic_reduce x y ->
+    forall m: @model _ (TrivialSemantics.SM Var), m |= x <-> m |= y.
+Proof.
+  intros; split; intros; destruct H; auto.
+Qed.
+
+Lemma sound_ReduceIff {Var: Type}:
+  forall x y: @expr (PropositionalLanguage.L Var),
+    ReduceIff.atomic_reduce x y ->
+    forall m: @model _ (TrivialSemantics.SM Var), m |= x <-> m |= y.
+Proof.
+  intros; split; intros; destruct H; auto.
+Qed.
+
+Lemma sound_ReduceTrueFalse {Var: Type}:
+  forall x y: @expr (PropositionalLanguage.L Var),
+    ReduceTrueFalse.atomic_reduce x y ->
+    forall m: @model _ (TrivialSemantics.SM Var), m |= x <-> m |= y.
+Proof.
+  intros; split; intros; destruct H.
+  + simpl in H0.
+    inversion H0.
+  + simpl; intro; auto.
+  + specialize (H0 I).
+    inversion H0.
+  + exact I.
+Qed.
+
+Lemma sound_disjunction {Var: Type}:
+  forall reduce1 reduce2: relation (@expr (PropositionalLanguage.L Var)),
+    (forall x y, reduce1 x y -> forall m: @model _ (TrivialSemantics.SM Var), m |= x <-> m |= y) ->
+    (forall x y, reduce2 x y -> forall m: @model _ (TrivialSemantics.SM Var), m |= x <-> m |= y) ->
+    (forall x y, relation_disjunction reduce1 reduce2 x y -> forall m: @model _ (TrivialSemantics.SM Var), m |= x <-> m |= y).
+Proof.
+  intros.
+  destruct H1.
+  + apply H; auto.
+  + apply H0; auto.
+Qed.
+
+Lemma sound_prop_congr {Var: Type}:
+  forall reduce: relation (@expr (PropositionalLanguage.L Var)),
+    (forall x y, reduce x y -> forall m: @model _ (TrivialSemantics.SM Var), m |= x <-> m |= y) ->
+    (forall x y, prop_congr reduce x y -> forall m: @model _ (TrivialSemantics.SM Var), m |= x <-> m |= y).
+Proof.
+  intros.
+  induction H0.
+  + apply H; auto.
+  + simpl in *.
+    unfold TrivialSemantics.sem_and, TrivialSemantics.sem_neg, TrivialSemantics.sem_imp; simpl.
+    tauto.
+  + simpl in *.
+    unfold TrivialSemantics.sem_or, TrivialSemantics.sem_neg, TrivialSemantics.sem_imp; simpl.
+    tauto.
+  + simpl in *.
+    unfold TrivialSemantics.sem_imp; simpl.
+    tauto.
+  + simpl in *.
+    unfold TrivialSemantics.sem_iff, TrivialSemantics.sem_and, TrivialSemantics.sem_neg, TrivialSemantics.sem_imp; simpl.
+    tauto.
+  + simpl in *.
+    unfold TrivialSemantics.sem_neg; simpl.
+    tauto.
+Qed.
+
+Lemma sound_clos_refl_trans {Var: Type}:
+  forall reduce: relation (@expr (PropositionalLanguage.L Var)),
+    (forall x y, reduce x y -> forall m: @model _ (TrivialSemantics.SM Var), m |= x <-> m |= y) ->
+    (forall x y, clos_refl_trans expr reduce x y -> forall m: @model _ (TrivialSemantics.SM Var), m |= x <-> m |= y).
+Proof.
+  intros.
+  induction H0.
+  + apply H; auto.
+  + tauto.
+  + tauto.
+Qed.
+
+Lemma sound_reduce {Var: Type}:
+  forall x y: @expr (PropositionalLanguage.L Var), reduce x y ->
+    forall m: @model _ (TrivialSemantics.SM Var), m |= x <-> m |= y.
+Proof.
+  apply sound_clos_refl_trans.
+  apply sound_prop_congr.
+  repeat apply sound_disjunction.
+  + apply sound_ImpNegAsPrime.
+  + apply sound_ReduceIff.
+  + apply sound_ReduceTrueFalse.
+Qed.
+
+Lemma sound_modus_ponens {Var: Type}:
+  forall x y: @expr (PropositionalLanguage.L Var),
+    forall m: @model _ (TrivialSemantics.SM Var),
+      m |= (x --> y) -> m |= x -> m |= y.
+Proof.
+  intros.
+  apply H; auto.
+Qed.
+
+Lemma sound_axiom1 {Var: Type}:
+  forall x y: @expr (PropositionalLanguage.L Var),
+    forall m: @model _ (TrivialSemantics.SM Var),
+      m |= x --> y --> x.
+Proof.
+  intros; intros ? ?; auto.
+Qed.
+
+Lemma sound_axiom2 {Var: Type}:
+  forall x y z: @expr (PropositionalLanguage.L Var),
+    forall m: @model _ (TrivialSemantics.SM Var),
+      m |= (x --> y --> z) --> (x --> y) --> (x --> z).
+Proof.
+  intros.
+  simpl.
+  intros ? ? ?.
+  specialize (H H1).
+  specialize (H0 H1).
+  auto.
+Qed.
+
+Lemma sound_axiom3 {Var: Type}:
+  forall x y: @expr (PropositionalLanguage.L Var),
+    forall m: @model _ (TrivialSemantics.SM Var),
+      m |= (~~ y --> x) --> (~~ y --> ~~ x) --> y.
+Proof.
+  intros.
+  simpl; intros ? ?.
+  destruct (Classical_Prop.classic (TrivialSemantics.denotation y m)); auto.
+  specialize (H H1).
+  specialize (H0 H1).
+  contradiction.
+Qed.
+
+Theorem sound_classical_trivial (Var: Type): sound (ClassicalPropositionalLogic.G Var) (TrivialSemantics.SM Var).
+Proof.
+  hnf; intros.
+  intro m.
+  induction H.
+  + pose proof sound_reduce x y H.
+    exact (proj1 (H1 m) IHprovable).
+  + pose proof sound_modus_ponens x y.
+    exact (H1 m IHprovable1 IHprovable2).
+  + apply sound_axiom1.
+  + apply sound_axiom2.
+  + apply sound_axiom3.
+Qed.
